core/RichTraceLink.v
@@ -46,54 +46,11 @@ Definition getName (tl: TraceLink):=
 Open Scope bool_scope.
 
 
-Definition source_compare (s:InputPiece * nat * string) (t:TraceLink) : bool :=
-  match s with 
-    (e,i,n) =>
-      list_beq tc.(SourceElement_eqb) (getSourcePiece t) e
-      && Nat.eqb (getIteration t) i
-      && String.eqb (getName t) n
-  end.
-
-
-
-Lemma source_compare_refl : 
-  (forall a,  SourceElement_eqb a a = true) ->
-  forall a b c, 
-    source_compare a {| source := a ; produced := b ; linkPattern := c |} = true.
-Proof.
-  intros R a b c.
-  destruct a as ((l & i) & n). 
-  simpl.
-  unfold getSourcePiece, getIteration, getName ; simpl.
-  rewrite list_beq_refl ; [ | exact R].
-  rewrite NPeano.Nat.eqb_refl.
-  rewrite String.eqb_refl. 
-  reflexivity.
-Qed.
-
-(* Not Used *)
-(* The requirement is too strong for the general case *)
-Lemma source_compare_correct :
-  (forall a b : Metamodel.ElementType SourceMetamodel,
-  Metamodel.elements_eqdec SourceMetamodel a b = true -> a = b) ->
-  forall a b,
-    source_compare a b = true -> b.(source) = a.
-Proof.
-  intro H1.
-  unfold source_compare.
-  intros a b H2 ; destruct a ; destruct p ; destruct b.
-  simpl. destruct source0 ; simpl in *.
-  BoolUtils.destruct_conjunctions.
-  destruct p ; simpl in *.
-  apply EqNat.beq_nat_true in H2 ; subst .
-  apply String.eqb_eq in H0 ; subst.
-  apply list_beq_correct in H ; subst.
-  + reflexivity.
-  + exact H1. 
-Qed.
-
 Definition convert (a:TraceLink) : PoorTraceLink.TraceLink :=
-  PoorTraceLink.buildTraceLink a.(source) a.(produced).
+  {| 
+    PoorTraceLink.source := a.(source) ;
+    PoorTraceLink.produced := a.(produced)
+  |}.
 
 Definition drop := map convert.
 
@@ -107,8 +64,6 @@ Qed.
 End TraceLink.
 
 Arguments TraceLink {_}.
-
-Arguments source_compare : simpl never.
 
 Notation Trace := (list TraceLink).
 
